src/pf2ir/FutureCertify.v
@@ -1,4 +1,5 @@
 Require Import RelationClasses.
+Require Import Coq.Logic.PropExtensionality.
 
 From sflib Require Import sflib.
 From Paco Require Import paco.
@@ -63,6 +64,14 @@ Module FutureCertify.
         (MAP2: f loc y fy),
         Time.lt x y.
 
+    Variant map_wf: Prop :=
+      | map_wf_intro
+          (MAP_EQ: map_eq)
+          (MAP_EQ_INV: map_eq_inv)
+          (MAP_LT: map_lt)
+          (MAP_LT_INV: map_lt_inv)
+    .
+
     Definition map_complete (mem fmem: Memory.t): Prop :=
       forall loc ts fts (MAP: f loc ts fts),
         (<<COMPLETE: exists from to msg,
@@ -71,15 +80,6 @@ Module FutureCertify.
         (<<FCOMPLETE: exists ffrom fto fmsg,
             (<<FGET: Memory.get loc fto fmem = Some (ffrom, fmsg)>>) /\
             (<<FTS: fts = ffrom \/ fts = fto>>)>>)
-    .
-
-    Variant map_wf (mem fmem: Memory.t): Prop :=
-      | map_wf_intro
-          (MAP_EQ: map_eq)
-          (MAP_EQ_INV: map_eq_inv)
-          (MAP_LT: map_lt)
-          (MAP_LT_INV: map_lt_inv)
-          (MAP_COMPLETE: map_complete mem fmem)
     .
 
     Definition timemap_map (tm ftm: TimeMap.t): Prop :=
@@ -116,7 +116,7 @@ Module FutureCertify.
 
     Variant memory_map_loc (loc: Loc.t) (max: Time.t): forall (rsv: bool) (mem fmem: Memory.t), Prop :=
       | memory_map_loc_reserved
-          f mem fmem
+          mem fmem
           fmax
           (SOUND: forall from to msg (GET: Memory.get loc to mem = Some (from, msg)),
             exists ffrom fto fmsg,
@@ -134,9 +134,9 @@ Module FutureCertify.
                 (<<FROM: f loc from ffrom>>) /\
                 (<<TO: f loc to fto>>) /\
                 (<<MSG: message_map msg fmsg>>)):
-        memory_map_loc loc max false mem fmem
+        memory_map_loc loc max true mem fmem
       | memory_map_loc_non_reserved
-          f mem fmem
+          mem fmem
           fmin
           (SOUND: forall from to msg (GET: Memory.get loc to mem = Some (from, msg)),
             exists ffrom fto fmsg,
@@ -161,22 +161,175 @@ Module FutureCertify.
       forall loc, memory_map_loc loc (max loc) (rsv loc) mem fmem.
   End FutureCertify.
 
+
+  Definition map_add (loc: Loc.t) (ts fts: Time.t) (f: map_t): map_t :=
+    fun loc' ts' fts' =>
+      (loc' = loc /\ ts' = ts /\ fts' = fts) \/ f loc' ts' fts'.
+
+  Lemma map_add_eq
+        (f: map_t) loc ts fts
+        (MAP: f loc ts fts):
+    map_add loc ts fts f = f.
+  Proof.
+    extensionality loc'.
+    extensionality ts'.
+    extensionality fts'.
+    apply propositional_extensionality.
+    unfold map_add.
+    split; auto. i. des; subst; ss.
+  Qed.
+
+  Lemma lt_get_from
+        mem loc
+        from1 to1 msg1
+        from2 to2 msg2
+        (LT: Time.lt to1 to2)
+        (GET1: Memory.get loc to1 mem = Some (from1, msg1))
+        (GET2: Memory.get loc to2 mem = Some (from2, msg2)):
+    Time.le to1 from2.
+  Proof.
+    exploit Memory.get_ts; try exact GET1. i. des.
+    { subst. timetac. }
+    exploit Memory.get_disjoint; [exact GET1|exact GET2|]. i. des.
+    { subst. timetac. }
+    destruct (TimeFacts.le_lt_dec to1 from2); ss. exfalso.
+    apply (x1 to1); econs; ss; try refl. econs. ss.
+  Qed.
+
+  Lemma add_cases
+        mem1 loc from to msg mem2
+        (INHABITED: Memory.inhabited mem1)
+        (ADD: Memory.add mem1 loc from to msg mem2):
+    exists pfrom pto pmsg,
+      (<<PGET: Memory.get loc pto mem1 = Some (pfrom, pmsg)>>) /\
+      (<<PREV_FROM: Time.le pto from>>) /\
+      (<<PREV_TO: Time.lt pto to>>) /\
+      (<<PEMPTY: Memory.empty mem1 loc pto to>>) /\
+      __guard__ (
+          (exists nfrom nto nmsg,
+              (<<NGET: Memory.get loc nto mem1 = Some (nfrom, nmsg)>>) /\
+              (<<NEXT_FROM: Time.le to nfrom>>) /\
+              (<<NEXT_TO: Time.lt to nto>>) /\
+              (<<NEMPTY: Memory.empty mem1 loc to nto>>)) \/
+          (<<LATEST: forall ts (LT: Time.lt to ts), Memory.get loc ts mem1 = None>>)).
+  Proof.
+    exploit Memory.add_ts; eauto. i.
+    hexploit Memory.add_inhabited; eauto. i. des.
+    exploit Memory.add_get0; eauto. i. des.
+    exploit (@Memory.prev_exists to mem2 loc); try apply H.
+    { eapply TimeFacts.le_lt_lt; eauto. apply Time.bot_spec. }
+    i. des.
+    revert x1. erewrite Memory.add_o; eauto. condtac; ss.
+    { des. subst. timetac. }
+    clear o COND. i.
+    esplits; try eapply x1; eauto.
+    { exploit Memory.add_get1; try exact x1; eauto. i.
+      eapply lt_get_from; eauto.
+    }
+    { ii. exploit x3; eauto.
+      erewrite Memory.add_o; eauto. condtac; ss.
+    }
+    destruct (TimeFacts.le_lt_dec (Memory.max_ts loc mem1) to).
+    { right. i.
+      destruct (Memory.get loc ts mem1) as [[]|] eqn:GET'; ss.
+      exploit Memory.max_ts_spec; try exact GET'. i. des.
+      rewrite l in MAX. timetac.
+    }
+    { left.
+      exploit Memory.next_exists; try exact l; eauto. i. des.
+      esplits; eauto.
+      exploit Memory.add_get1; try exact x6; eauto. i.
+      eapply lt_get_from; eauto.
+    }
+  Qed.
+
   Lemma memory_map_add
         f1 max rsv mem1 fmem1
         loc from to msg mem2
         fmsg
+        (WF1: map_wf f1)
+        (COMPLETE1: map_complete f1 mem1 fmem1)
         (MAP1: memory_map f1 max rsv mem1 fmem1)
-        (WF1: map_wf f1 mem1 fmem1)
+        (INHABITED1: Memory.inhabited mem1)
         (ADD: Memory.add mem1 loc from to msg mem2)
-        (RESERVE: rsv loc = false -> Time.lt (max loc) from):
-    exists f2 ffrom fto fmem2,
-      (<<FADD: Memory.add fmem1 loc ffrom fto fmsg fmem2>>) /\
+        (RESERVE: rsv loc = false -> Time.lt (max loc) from)
+        (MSG_WF: Message.wf fmsg):
+    exists ffrom fto f2 fmem2,
       (<<F2: f2 = fun loc' ts fts =>
                     (loc' = loc /\ ts = to /\ fts = fto) \/
                     (loc' = loc /\ ts = from /\ fts = ffrom) \/
                     f1 loc' ts fts>>) /\
-      (<<MAP2: message_map f2 msg fmsg -> memory_map f2 max rsv mem2 fmem2>>) /\
-      (<<WF2: map_wf f2 mem2 fmem2>>).
+      (<<FADD: Memory.add fmem1 loc ffrom fto fmsg fmem2>>) /\
+      (<<WF2: map_wf f2>>) /\
+      (<<COMPLETE2: map_complete f2 mem2 fmem2>>) /\
+      (<<MAP2: message_map f2 msg fmsg -> memory_map f2 max rsv mem2 fmem2>>).
   Proof.
+    inv WF1.
+    exploit Memory.add_ts; eauto. intro TS.
+    exploit add_cases; eauto. i. des.
+    destruct (rsv loc) eqn:RSV.
+    { (* reserved *)
+      destruct (MAP1 loc); ss.
+      unguard. des.
+
+      { (* non-latest *)
+        exploit Memory.get_ts; try exact NGET. i. des; subst; timetac.
+        assert (Time.lt pto nfrom).
+        { eapply TimeFacts.lt_le_lt; try exact PREV_TO. ss. }
+        exploit SOUND; try exact PGET. i. des.
+        rename ffrom into fpfrom, fto into fpto, fmsg0 into fpmsg.
+        exploit SOUND; try exact NGET. i. des.
+        rename ffrom into fnfrom, fto into fnto, fmsg0 into fnmsg.
+        assert (exists fto,
+                   (<<FPREV_TO: Time.lt fpto fto>>) /\
+                   (<<FNEXT_FROM: Time.le fto fnfrom>>) /\
+                   (<<FNEXT_TO: Time.lt fto fnto>>) /\
+                   (<<NEXT_EQ: __guard__ (to = nfrom <-> fto = fnfrom)>>)).
+        { inv NEXT_FROM.
+          - exploit MAP_LT; try exact H; eauto. i.
+            exists (Time.middle fpto fnfrom).
+            exploit Time.middle_spec; try exact x1. i. des.
+            unguard. splits; ss.
+            + econs. ss.
+            + etrans; try exact x3. eapply MAP_LT; try exact x0; eauto.
+            + split; i; subst; timetac.
+              rewrite <- H1 in x3 at 2. timetac.
+          - inv H0. exists fnfrom. unguard. splits; ss.
+            + eapply MAP_LT; try exact H; eauto.
+            + refl.
+            + eapply MAP_LT; try exact x0; eauto.
+        }
+        des.
+        assert (exists ffrom,
+                   (<<FTS: Time.lt ffrom fto>>) /\
+                   (<<FPREV_FROM: Time.le fpto ffrom>>) /\
+                   (<<PREV_EQ: __guard__ (pto = from <-> fpto = ffrom)>>)).
+        { inv PREV_FROM.
+          - exists (Time.middle fpto fto).
+            exploit Time.middle_spec; try exact FPREV_TO. i. des.
+            unguard. splits; ss.
+            + econs. ss.
+            + split; i; subst; timetac.
+              rewrite H1 in x1 at 1. timetac.
+          - inv H0. exists fpto. unguard. splits; ss. refl.
+        }
+        des.
+        exploit (@Memory.add_exists fmem loc); try exact FTS; try exact MSG_WF.
+        { admit.
+        }
+        i. des. esplits; try exact x1; eauto; try refl.
+        - admit.
+        - admit.
+        - admit.
+      }
+
+      { (* latest *)
+        admit.
+      }
+    }
+
+    { (* non-reserved *)
+      admit.
+    }
   Admitted.
 End FutureCertify.
